\documentclass[12pt]{article}

 
\newcommand{\N}{\mathbb{N}}
\newcommand{\Z}{\mathbb{Z}}
\usepackage{amsmath,amsthm,amssymb,pdfpages}


\begin{document}
 
\title{Zombie model with human behavior equations}
\author{Luke Botti\\
Course number: MATH 502}
\maketitle
 
$$\frac{dS}{dt} = bS(t) - mS(t) -\alpha S(t)Z(t) + r(Q(t)+E(t))$$

$$C(t) = \begin{cases}
	0 & Q(t) < q_{\text{max}} \vee X_S(t) < 1/2 \\
	C_0 & Q(t) \geq q_{\text{max}} \wedge X_S(t) \geq 1/2
\end{cases}$$

$$\frac{dE}{dt} = \begin{cases} 
      \alpha S(t)Z(t) - zE(t) -rE(t) - (C_0 + X_E(t))E(t) - C(t) E(t) & Q(t) < q_{\text{max}} \\
      \alpha S(t)Z(t) - zE(t) -rE(t) - C(t) E(t) & Q(t) \geq q_{\text{max}}
   \end{cases}
$$

$$\frac{dQ}{dt} = \begin{cases}
	(C_0 + X_E)E - rQ(t) - zQ(t) & Q(t) < q_{\text{max}}\\
	-rQ(t) - zQ(t) & Q(t) \geq q_{\text{max}}
\end{cases}$$

$$\frac{dZ}{dt} = zE(t) -kS(t)Z(t)$$

$$\frac{dD}{dt} = kS(t)Z(t) + mS(t) + zQ(t) + C(t)E$$

$$\frac{dX_S}{dt} = k_S X_S(t) (1 - X_S(t))[Z(t) + Q(t) - \epsilon_S L_S(t)]$$

$$\frac{dX_E}{dt} = k_E X_E(t) (1 - X_E(t))\{(z-r)[E(t) + Q(t)] - \epsilon_E\}$$

$$\frac{dL_S}{dt} = \beta C(t) - \mu L_s(t)$$





\end{document}